proofs/fstar/extraction/Ristretto255.Constants.fst
@@ -3,36 +3,6 @@ module Ristretto255.Constants
 open FStar.Mul
 open Core_models
 
-/// Edwards `d` value, equal to `-121665/121666 mod p`.
-let v_EDWARDS_D: Ristretto255.Field.t_FieldElement =
-  Ristretto255.Field.FieldElement
-  (let list =
-      [
-        mk_u64 929955233495203;
-        mk_u64 466365720129213;
-        mk_u64 1662059464998953;
-        mk_u64 2033849074728123;
-        mk_u64 1442794654840575
-      ]
-    in
-    FStar.Pervasives.assert_norm (Prims.eq2 (List.Tot.length list) 5);
-    Rust_primitives.Hax.array_of_list 5 list)
-  <:
-  Ristretto255.Field.t_FieldElement
+include Ristretto255.Bundle {v_EDWARDS_D as v_EDWARDS_D}
 
-/// Precomputed value of one of the square roots of -1 (mod p).
-let v_SQRT_M1: Ristretto255.Field.t_FieldElement =
-  Ristretto255.Field.FieldElement
-  (let list =
-      [
-        mk_u64 1718705420411056;
-        mk_u64 234908883556509;
-        mk_u64 2233514472574048;
-        mk_u64 2117202627021982;
-        mk_u64 765476049583133
-      ]
-    in
-    FStar.Pervasives.assert_norm (Prims.eq2 (List.Tot.length list) 5);
-    Rust_primitives.Hax.array_of_list 5 list)
-  <:
-  Ristretto255.Field.t_FieldElement
+include Ristretto255.Bundle {v_SQRT_M1 as v_SQRT_M1}
