proofs/fstar/extraction/Ristretto255.fst
@@ -3,38 +3,38 @@ module Ristretto255
 open FStar.Mul
 open Core_models
 
-include Ristretto255.Bundle {t_CompressedRistretto as t_CompressedRistretto}
+include Ristretto255.Bundle_decompress {t_CompressedRistretto as t_CompressedRistretto}
 
-include Ristretto255.Bundle {CompressedRistretto as CompressedRistretto}
+include Ristretto255.Bundle_decompress {CompressedRistretto as CompressedRistretto}
 
-include Ristretto255.Bundle {impl_2 as impl_2}
+include Ristretto255.Bundle_decompress {impl_2 as impl_2}
 
-include Ristretto255.Bundle {impl_3 as impl_3}
+include Ristretto255.Bundle_decompress {impl_3 as impl_3}
 
-include Ristretto255.Bundle {impl_4 as impl_4}
+include Ristretto255.Bundle_decompress {impl_4 as impl_4}
 
-include Ristretto255.Bundle {impl_5 as impl_5}
+include Ristretto255.Bundle_decompress {impl_5 as impl_5}
 
-include Ristretto255.Bundle {impl_6 as impl_6}
+include Ristretto255.Bundle_decompress {impl_6 as impl_6}
 
-include Ristretto255.Bundle {impl_7 as impl_7}
+include Ristretto255.Bundle_decompress {impl_7 as impl_7}
 
-include Ristretto255.Bundle {impl_8__to_bytes as impl_CompressedRistretto__to_bytes}
+include Ristretto255.Bundle_decompress {impl_8__to_bytes as impl_CompressedRistretto__to_bytes}
 
-include Ristretto255.Bundle {impl_8__as_bytes as impl_CompressedRistretto__as_bytes}
+include Ristretto255.Bundle_decompress {impl_8__as_bytes as impl_CompressedRistretto__as_bytes}
 
-include Ristretto255.Bundle {impl_8__from_slice as impl_CompressedRistretto__from_slice}
+include Ristretto255.Bundle_decompress {impl_8__from_slice as impl_CompressedRistretto__from_slice}
 
-include Ristretto255.Bundle {impl_8__decompress as impl_CompressedRistretto__decompress}
+include Ristretto255.Bundle_decompress {impl_8__decompress as impl_CompressedRistretto__decompress}
 
-include Ristretto255.Bundle {impl as impl}
+include Ristretto255.Bundle_decompress {impl as impl}
 
-include Ristretto255.Bundle {impl_1 as impl_1}
+include Ristretto255.Bundle_decompress {impl_1 as impl_1}
 
-include Ristretto255.Bundle {impl_9 as impl_9}
+include Ristretto255.Bundle_decompress {impl_9 as impl_9}
 
-include Ristretto255.Bundle {t_RistrettoPoint as t_RistrettoPoint}
+include Ristretto255.Bundle_decompress {t_RistrettoPoint as t_RistrettoPoint}
 
-include Ristretto255.Bundle {RistrettoPoint as RistrettoPoint}
+include Ristretto255.Bundle_decompress {RistrettoPoint as RistrettoPoint}
 
-include Ristretto255.Bundle {t_EdwardsPoint as t_EdwardsPoint}
+include Ristretto255.Bundle_decompress {t_EdwardsPoint as t_EdwardsPoint}
